thy/Iptables_Semantics/Examples/Code_haskell.thy
@@ -42,7 +42,7 @@ export_code Rule
   mk_ipv6addr IPv6AddrPreferred ipv6preferred_to_int int_to_ipv6preferred
   ipt_ipv6range_toString
   common_primitive_v6_toString
-  (**)
+  sanity_check_simple_firewall
   common_primitive_match_expr_toString
   simple_rule_toString
   Semantics_Goto.rewrite_Goto_safe
@@ -55,6 +55,8 @@ export_code Rule
   to_simple_firewall_without_interfaces
   sanity_wf_ruleset
   has_default_policy
+  (*sanity checking the simple firewall*)
+  
   (*spoofing:*) ipassmt_generic
   no_spoofing_iface ipassmt_sanity_defined map_of_ipassmt to_ipassmt debug_ipassmt
   Pos Neg
