thy/Iptables_Semantics/Examples/Parser_Test/Parser6_Test.thy
@@ -17,10 +17,12 @@ thm parser_test_firewall_FORWARD_default_policy_def
 
 value[code] "parser_test_firewall"
 
-
-value[code] "map quote_rewrite
+lemma "sanity_check_simple_firewall
+              (to_simple_firewall (upper_closure
+                (optimize_matches abstract_for_simple_firewall
+                  (upper_closure (packet_assume_new
                     (unfold_ruleset_FORWARD parser_test_firewall_FORWARD_default_policy
-                      (map_of parser_test_firewall))))"
+                      (map_of parser_test_firewall))))))) = False" by eval
 
 value[code] "map simple_rule6_toString
               (to_simple_firewall (upper_closure
@@ -29,6 +31,53 @@ value[code] "map simple_rule6_toString
                     (unfold_ruleset_FORWARD parser_test_firewall_FORWARD_default_policy
                       (map_of parser_test_firewall)))))))" 
 (*33.224s*)
+
+text\<open>here is a minimal example\<close>
+value[code] " (unfold_ruleset_FORWARD action.Accept
+                      (map_of_string_ipv4
+                              [(''FORWARD'', [Rule MatchAny (Call ''CHAIN'')]),
+                               (''CHAIN'',
+                                [Rule (MatchAnd (Match (Prot (Proto TCP)))
+                                        (Match (Src_Ports [(22, 22)])))
+                                  Return,
+                                 Rule (MatchAnd (Match (Prot (Proto UDP)))
+                                        (Match (Dst_Ports [(80,80)])))
+                                  Return,
+                                 Rule MatchAny action.Drop])
+                              ]))"
+
+
+value[code] "map simple_rule_toString
+              (to_simple_firewall (upper_closure
+                (optimize_matches abstract_for_simple_firewall
+                  (upper_closure (packet_assume_new
+                    (unfold_ruleset_FORWARD parser_test_firewall_FORWARD_default_policy
+                      (map_of_string_ipv4 [(''FORWARD'', [Rule MatchAny (Call ''CHAIN'')]),
+                               (''CHAIN'',
+                                [Rule (MatchAnd (Match (Prot (Proto TCP)))
+                                        (Match (Src_Ports [(22, 22)])))
+                                  Return,
+                                 Rule (MatchAnd (Match (Prot (Proto UDP)))
+                                        (Match (Dst_Ports [(80,80)])))
+                                  Return,
+                                 Rule MatchAny action.Drop])
+                              ])))))))" 
+
+lemma "sanity_check_simple_firewall
+              (to_simple_firewall (upper_closure
+                (optimize_matches abstract_for_simple_firewall
+                  (upper_closure (packet_assume_new
+                    (unfold_ruleset_FORWARD parser_test_firewall_FORWARD_default_policy
+                      (map_of_string_ipv4 [(''FORWARD'', [Rule MatchAny (Call ''CHAIN'')]),
+                               (''CHAIN'',
+                                [Rule (MatchAnd (Match (Prot (Proto TCP)))
+                                        (Match (Src_Ports [(22, 22)])))
+                                  Return,
+                                 Rule (MatchAnd (Match (Prot (Proto UDP)))
+                                        (Match (Dst_Ports [(80,80)])))
+                                  Return,
+                                 Rule MatchAny action.Drop])
+                              ]))))))) = False" by eval 
 
 (*
 
