thy/Iptables_Semantics/Examples/medium-sized-company/Analyze_medium_sized_company.thy
@@ -60,7 +60,13 @@ value[code] "map simple_rule_toString (to_simple_firewall
 value[code] "map simple_rule_toString (to_simple_firewall
     (lower_closure (optimize_matches abstract_for_simple_firewall (lower_closure (packet_assume_new unfolded_FORWARD)))))"
 
+lemma "sanity_check_simple_firewall (to_simple_firewall
+    (upper_closure (optimize_matches abstract_for_simple_firewall (upper_closure (packet_assume_new unfolded_FORWARD)))))"
+  by eval
 
+lemma "sanity_check_simple_firewall (to_simple_firewall
+    (lower_closure (optimize_matches abstract_for_simple_firewall (lower_closure (packet_assume_new unfolded_FORWARD)))))"
+  by eval
 (*
 text{*If we call the IP address spcae partitioning incorrectly (not prepocessed, still has interfaces), we get an error*}
 value[code] " parts_connection_ssh 
