thy/Iptables_Semantics/Examples/topoS_generated/Analyze_topos_generated.thy
@@ -47,6 +47,13 @@ value[code] "upper_closure (packet_assume_new unfolded_FORWARD)"
 lemma "check_simple_fw_preconditions (upper_closure (optimize_matches abstract_for_simple_firewall 
           (upper_closure (packet_assume_new unfolded_FORWARD))))" by eval
 
+lemma "simple_fw_valid (to_simple_firewall (upper_closure
+              (optimize_matches abstract_for_simple_firewall (upper_closure (packet_assume_new unfolded_FORWARD)))))"
+by eval
+lemma "simple_fw_valid (to_simple_firewall (lower_closure
+              (optimize_matches abstract_for_simple_firewall (lower_closure (packet_assume_new unfolded_FORWARD)))))"
+by eval
+
 
 value[code] "map simple_rule_toString (to_simple_firewall (upper_closure
               (optimize_matches abstract_for_simple_firewall (upper_closure (packet_assume_new unfolded_FORWARD)))))"
